clean up CStanSemanticsTarget

stanfrontend/CStanSemanticsBackend.v
@@ -13,6 +13,7 @@ Require Import Ctypes.
 Require Import Cop.
 
 Require Import CStan.
+Require Import CStanCont.
 
 Section SEMANTICS.
 
@@ -171,38 +172,6 @@ Inductive eval_exprlist: list expr -> typelist -> list val -> Prop :=
 End EXPR.
 
 (** ** Transition semantics for statements and functions *)
-
-(** Continuations *)
-
-Inductive cont: Type :=
-  | Kstop: cont
-  | Kseq: statement -> cont -> cont       (**r [Kseq s2 k] = after [s1] in [s1;s2] *)
-  | Kloop1: statement -> statement -> cont -> cont (**r [Kloop1 s1 s2 k] = after [s1] in [Sloop s1 s2] *)
-  | Kloop2: statement -> statement -> cont -> cont (**r [Kloop1 s1 s2 k] = after [s2] in [Sloop s1 s2] *)
-  | Kswitch: cont -> cont       (**r catches [break] statements arising out of [switch] *)
-  | Kcall: option ident ->                  (**r where to store result *)
-           function ->                      (**r calling function *)
-           env ->                           (**r local env of calling function *)
-           temp_env ->                      (**r temporary env of calling function *)
-           cont -> cont.
-
-(** Pop continuation until a call or stop *)
-
-Fixpoint call_cont (k: cont) : cont :=
-  match k with
-  | Kseq s k => call_cont k
-  | Kloop1 s1 s2 k => call_cont k
-  | Kloop2 s1 s2 k => call_cont k
-  | Kswitch k => call_cont k
-  | _ => k
-  end.
-
-Definition is_call_cont (k: cont) : Prop :=
-  match k with
-  | Kstop => True
-  | Kcall _ _ _ _ _ => True
-  | _ => False
-  end.
 
 Inductive state: Type :=
   | State                               (**r execution of a statement *)
