stanfrontend/CStanCont.v
@@ -1,0 +1,35 @@
+Require Import AST.
+Require Import CStan.
+
+(** Continuations *)
+
+Inductive cont: Type :=
+  | Kstop: cont
+  | Kseq: statement -> cont -> cont       (**r [Kseq s2 k] = after [s1] in [s1;s2] *)
+  | Kloop1: statement -> statement -> cont -> cont (**r [Kloop1 s1 s2 k] = after [s1] in [Sloop s1 s2] *)
+  | Kloop2: statement -> statement -> cont -> cont (**r [Kloop1 s1 s2 k] = after [s2] in [Sloop s1 s2] *)
+  | Kswitch: cont -> cont       (**r catches [break] statements arising out of [switch] *)
+  | Kcall: option ident ->                  (**r where to store result *)
+           function ->                      (**r calling function *)
+           env ->                           (**r local env of calling function *)
+           temp_env ->                      (**r temporary env of calling function *)
+           cont -> cont.
+
+(** Pop continuation until a call or stop *)
+
+Fixpoint call_cont (k: cont) : cont :=
+  match k with
+  | Kseq s k => call_cont k
+  | Kloop1 s1 s2 k => call_cont k
+  | Kloop2 s1 s2 k => call_cont k
+  | Kswitch k => call_cont k
+  | _ => k
+  end.
+
+Definition is_call_cont (k: cont) : Prop :=
+  match k with
+  | Kstop => True
+  | Kcall _ _ _ _ _ => True
+  | _ => False
+  end.
+
